c_stubs/tls13_record_for_flight_state.h
@@ -1,0 +1,12 @@
+#ifndef TLS13_RECORD_FOR_FLIGHT_STATE_H
+#define TLS13_RECORD_FOR_FLIGHT_STATE_H
+
+#include "TLS13_Record.h"
+
+#define TLS13_Record_record_state_free(st, erased) TLS13_Record_record_state_free(st)
+#define TLS13_Record_install_handshake_keys_runtime(st, key, iv, erased_st, key_bytes, iv_bytes) \
+    TLS13_Record_install_handshake_keys_runtime(st, key, iv)
+#define TLS13_Record_open_application_runtime(st, aad, aad_len, cipher, cipher_len, out, erased_st, aad_bytes, cipher_bytes, old_out) \
+    TLS13_Record_open_application_runtime(st, aad, aad_len, cipher, cipher_len, out)
+
+#endif
